Docs/ContextualEmbedding/package.lean
@@ -1,5 +1,4 @@
 import «ContextualEmbedding».CE
-import «ContextualEmbedding».CEEval
 import «ContextualEmbedding».CEEval_Alt
 import «ContextualEmbedding».__CEFnExample
 import «ContextualEmbedding».«1_CleanUpIndex».CE
